test262/RegexpTree.ml
@@ -1,7 +1,4 @@
 open Yojson
-open Warblre.Interop
-open Warblre.Extracted.Patterns
-open Warblre.Extracted.ECMA
 
 let find_field ls name = let (_, r) = List.find (fun (n, _) -> String.equal n name) ls in r
 
@@ -9,178 +6,369 @@ let reduce_left f ls = match ls with
   | h :: t -> List.fold_left f h t
   | _ -> failwith "Cannot reduce empty list"
 
-let json_to_regex (json: (string * Yojson.Safe.t) list) index: coq_RegExpInstance =
-  Yojson.Safe.(
-    let iter_ca (json: Yojson.Safe.t): coq_ClassAtom = (match json with
-    | `Assoc (("type", `String "Char") :: ("value", `String _) :: ("kind", `String "simple") :: ("symbol", `String _) :: ("codePoint", `Int codepoint) :: ("escaped", `Bool true) :: []) ->
-       ClassEsc (CCharacterEsc (IdentityEsc (Obj.magic (Warblre.Interop.char_of_int (Obj.magic codepoint)))))
-    | `Assoc (("type", `String "Char") :: ("value", `String _) :: ("kind", `String "simple") :: ("symbol", `String _) :: ("codePoint", `Int codepoint) :: []) ->
-      SourceCharacter ((Obj.magic (Warblre.Interop.char_of_int (Obj.magic codepoint))))
-    | `Assoc (("type", `String "Char") :: ("value", `String _) :: ("kind", `String "unicode") :: ("symbol", `String _) :: ("codePoint", `Int codepoint) :: []) ->
-      SourceCharacter ((Obj.magic (Warblre.Interop.char_of_int (Obj.magic codepoint))))
+module Utf16 = struct
+  open Warblre.Extracted.Patterns
+  open Warblre.Extracted.ECMA
+  open Warblre.Interop.Utf16
 
-    | `Assoc (("type", `String "Char") :: ("value", `String "\\b") :: ("kind", `String "meta") :: ("symbol", `String ".") :: ("codePoint", `Null) :: []) ->
-      ClassEsc(Coq_esc_b)
-    | `Assoc (("type", `String "Char") :: ("value", `String "\\s") :: ("kind", `String "meta") :: ("codePoint", `Null) :: []) ->
-      ClassEsc (CCharacterClassEsc (Coq_esc_s))
-    | `Assoc (("type", `String "Char") :: ("value", `String "\\d") :: ("kind", `String "meta") :: ("codePoint", `Null) :: []) ->
-      ClassEsc (CCharacterClassEsc (Coq_esc_d))
-    | `Assoc (("type", `String "Char") :: ("value", `String "\\w") :: ("kind", `String "meta") :: ("codePoint", `Null) :: []) ->
-      ClassEsc (CCharacterClassEsc (Coq_esc_w))
-    | `Assoc (("type", `String "Char") :: ("value", `String "\\S") :: ("kind", `String "meta") :: ("codePoint", `Null) :: []) ->
-      ClassEsc (CCharacterClassEsc (Coq_esc_S))
-    | `Assoc (("type", `String "Char") :: ("value", `String "\\D") :: ("kind", `String "meta") :: ("codePoint", `Null) :: []) ->
-      ClassEsc (CCharacterClassEsc (Coq_esc_D))
-    | `Assoc (("type", `String "Char") :: ("value", `String "\\W") :: ("kind", `String "meta") :: ("codePoint", `Null) :: []) ->
-      ClassEsc (CCharacterClassEsc (Coq_esc_W))
+  let json_to_regex (json: (string * Yojson.Safe.t) list) index: coq_RegExpInstance =
+    Yojson.Safe.(
+      let iter_ca (json: Yojson.Safe.t): coq_ClassAtom = (match json with
+      | `Assoc (("type", `String "Char") :: ("value", `String _) :: ("kind", `String "simple") :: ("symbol", `String _) :: ("codePoint", `Int codepoint) :: ("escaped", `Bool true) :: []) ->
+        ClassEsc (CCharacterEsc (IdentityEsc (Obj.magic (char_of_int codepoint))))
+      | `Assoc (("type", `String "Char") :: ("value", `String _) :: ("kind", `String "simple") :: ("symbol", `String _) :: ("codePoint", `Int codepoint) :: []) ->
+        SourceCharacter ((Obj.magic (char_of_int codepoint)))
+      | `Assoc (("type", `String "Char") :: ("value", `String _) :: ("kind", `String "unicode") :: ("symbol", `String _) :: ("codePoint", `Int codepoint) :: []) ->
+        SourceCharacter ((Obj.magic (char_of_int codepoint)))
 
-    | `Assoc (("type", `String "Char") :: ("value", `String "\\t") :: ("kind", `String "meta") :: ("symbol", `String _) :: ("codePoint", `Int _) :: []) ->
-      ClassEsc (CCharacterEsc (ControlEsc (Coq_esc_t)))
-    | `Assoc (("type", `String "Char") :: ("value", `String "\\n") :: ("kind", `String "meta") :: ("symbol", `String _) :: ("codePoint", `Int _) :: []) ->
-      ClassEsc (CCharacterEsc (ControlEsc (Coq_esc_n)))
-    | `Assoc (("type", `String "Char") :: ("value", `String "\\f") :: ("kind", `String "meta") :: ("symbol", `String _) :: ("codePoint", `Int _) :: []) ->
-      ClassEsc (CCharacterEsc (ControlEsc (Coq_esc_f)))
-    | `Assoc (("type", `String "Char") :: ("value", `String "\\v") :: ("kind", `String "meta") :: ("symbol", `String _) :: ("codePoint", `Int _) :: []) ->
-      ClassEsc (CCharacterEsc (ControlEsc (Coq_esc_v)))
-    | `Assoc (("type", `String "Char") :: ("value", `String "\\r") :: ("kind", `String "meta") :: ("symbol", `String _) :: ("codePoint", `Int _) :: []) ->
-      ClassEsc (CCharacterEsc (ControlEsc (Coq_esc_r)))
+      | `Assoc (("type", `String "Char") :: ("value", `String "\\b") :: ("kind", `String "meta") :: ("symbol", `String ".") :: ("codePoint", `Null) :: []) ->
+        ClassEsc(Coq_esc_b)
+      | `Assoc (("type", `String "Char") :: ("value", `String "\\s") :: ("kind", `String "meta") :: ("codePoint", `Null) :: []) ->
+        ClassEsc (CCharacterClassEsc (Coq_esc_s))
+      | `Assoc (("type", `String "Char") :: ("value", `String "\\d") :: ("kind", `String "meta") :: ("codePoint", `Null) :: []) ->
+        ClassEsc (CCharacterClassEsc (Coq_esc_d))
+      | `Assoc (("type", `String "Char") :: ("value", `String "\\w") :: ("kind", `String "meta") :: ("codePoint", `Null) :: []) ->
+        ClassEsc (CCharacterClassEsc (Coq_esc_w))
+      | `Assoc (("type", `String "Char") :: ("value", `String "\\S") :: ("kind", `String "meta") :: ("codePoint", `Null) :: []) ->
+        ClassEsc (CCharacterClassEsc (Coq_esc_S))
+      | `Assoc (("type", `String "Char") :: ("value", `String "\\D") :: ("kind", `String "meta") :: ("codePoint", `Null) :: []) ->
+        ClassEsc (CCharacterClassEsc (Coq_esc_D))
+      | `Assoc (("type", `String "Char") :: ("value", `String "\\W") :: ("kind", `String "meta") :: ("codePoint", `Null) :: []) ->
+        ClassEsc (CCharacterClassEsc (Coq_esc_W))
 
-    | `Assoc (("type", `String "Char") :: ("value", `String ctrl) :: ("kind", `String "control") :: []) ->
-      assert(String.length ctrl == 3);
-      ClassEsc (CCharacterEsc (AsciiControlEsc (String.get ctrl 2)))
-    | `Assoc (("type", `String "Char") :: ("value", `String hex) :: ("kind", `String "hex") :: ("symbol", `String _) :: ("codePoint", `Int _) :: []) ->
-      assert(String.length hex == 4);
-      ClassEsc (CCharacterEsc (HexEscape (String.get hex 2, String.get hex 3)))
+      | `Assoc (("type", `String "Char") :: ("value", `String "\\t") :: ("kind", `String "meta") :: ("symbol", `String _) :: ("codePoint", `Int _) :: []) ->
+        ClassEsc (CCharacterEsc (ControlEsc (Coq_esc_t)))
+      | `Assoc (("type", `String "Char") :: ("value", `String "\\n") :: ("kind", `String "meta") :: ("symbol", `String _) :: ("codePoint", `Int _) :: []) ->
+        ClassEsc (CCharacterEsc (ControlEsc (Coq_esc_n)))
+      | `Assoc (("type", `String "Char") :: ("value", `String "\\f") :: ("kind", `String "meta") :: ("symbol", `String _) :: ("codePoint", `Int _) :: []) ->
+        ClassEsc (CCharacterEsc (ControlEsc (Coq_esc_f)))
+      | `Assoc (("type", `String "Char") :: ("value", `String "\\v") :: ("kind", `String "meta") :: ("symbol", `String _) :: ("codePoint", `Int _) :: []) ->
+        ClassEsc (CCharacterEsc (ControlEsc (Coq_esc_v)))
+      | `Assoc (("type", `String "Char") :: ("value", `String "\\r") :: ("kind", `String "meta") :: ("symbol", `String _) :: ("codePoint", `Int _) :: []) ->
+        ClassEsc (CCharacterEsc (ControlEsc (Coq_esc_r)))
 
-    | _  -> failwith (String.cat "Unsupported JSON class atom: " (Yojson.Safe.show json)))
-    in
+      | `Assoc (("type", `String "Char") :: ("value", `String ctrl) :: ("kind", `String "control") :: []) ->
+        assert(String.length ctrl == 3);
+        ClassEsc (CCharacterEsc (AsciiControlEsc (String.get ctrl 2)))
+      | `Assoc (("type", `String "Char") :: ("value", `String hex) :: ("kind", `String "hex") :: ("symbol", `String _) :: ("codePoint", `Int _) :: []) ->
+        assert(String.length hex == 4);
+        ClassEsc (CCharacterEsc (HexEscape (String.get hex 2, String.get hex 3)))
 
-
-    let rec iter_cc (json: Yojson.Safe.t list): coq_ClassRanges = (match json with
-    | `Assoc (("type", `String "Char") :: r) :: t -> ClassAtomCR (iter_ca (`Assoc (("type", `String "Char") :: r)), iter_cc t)
-
-    | `Assoc (("type", `String "ClassRange") :: ("from", from) :: ("to", until) :: []) :: t->
-      RangeCR (iter_ca from, iter_ca until, iter_cc t)
-
-    | h :: _ -> failwith (String.cat "Unsupported JSON class ranges: " (Yojson.Safe.show h))
-    | [] -> EmptyCR)
-    in
+      | _  -> failwith (String.cat "Unsupported JSON class atom: " (Yojson.Safe.show json)))
+      in
 
 
-    let iter_quantifier (json: Yojson.Safe.t): coq_Quantifier = (match json with
-    | `Assoc (("type", `String "Quantifier") :: ("kind", `String "?") :: ("greedy", `Bool true) :: []) -> Greedy (Question)
-    | `Assoc (("type", `String "Quantifier") :: ("kind", `String "*") :: ("greedy", `Bool true) :: []) -> Greedy (Star)
-    | `Assoc (("type", `String "Quantifier") :: ("kind", `String "+") :: ("greedy", `Bool true) :: []) -> Greedy (Plus)
-    | `Assoc (("type", `String "Quantifier") :: ("kind", `String "Range") :: ("from", `Int from) :: ("greedy", `Bool true) :: []) -> Greedy (RepPartialRange (from))
-    | `Assoc (("type", `String "Quantifier") :: ("kind", `String "Range") :: ("from", `Int from) :: ("to", `Int until) :: ("greedy", `Bool true) :: []) -> Greedy (RepRange (from, until))
+      let rec iter_cc (json: Yojson.Safe.t list): coq_ClassRanges = (match json with
+      | `Assoc (("type", `String "Char") :: r) :: t -> ClassAtomCR (iter_ca (`Assoc (("type", `String "Char") :: r)), iter_cc t)
 
-    | `Assoc (("type", `String "Quantifier") :: ("kind", `String "?") :: ("greedy", `Bool false) :: []) -> Lazy (Question)
-    | `Assoc (("type", `String "Quantifier") :: ("kind", `String "*") :: ("greedy", `Bool false) :: []) -> Lazy (Star)
-    | `Assoc (("type", `String "Quantifier") :: ("kind", `String "+") :: ("greedy", `Bool false) :: []) -> Lazy (Plus)
-    | `Assoc (("type", `String "Quantifier") :: ("kind", `String "Range") :: ("from", `Int from) :: ("greedy", `Bool false) :: []) -> Lazy (RepPartialRange (from))
-    | `Assoc (("type", `String "Quantifier") :: ("kind", `String "Range") :: ("from", `Int from) :: ("to", `Int until) :: ("greedy", `Bool false) :: []) -> Lazy (RepRange (from, until))
+      | `Assoc (("type", `String "ClassRange") :: ("from", from) :: ("to", until) :: []) :: t->
+        RangeCR (iter_ca from, iter_ca until, iter_cc t)
 
-    | _ -> failwith (String.cat "Unsupported JSON class ranges: " (Yojson.Safe.show json)))
-    in
+      | h :: _ -> failwith (String.cat "Unsupported JSON class ranges: " (Yojson.Safe.show h))
+      | [] -> EmptyCR)
+      in
 
 
-    let rec iter_r (json: Yojson.Safe.t): coq_Regex = (match json with
-    | `Null -> Empty
+      let iter_quantifier (json: Yojson.Safe.t): coq_Quantifier = (match json with
+      | `Assoc (("type", `String "Quantifier") :: ("kind", `String "?") :: ("greedy", `Bool true) :: []) -> Greedy (Question)
+      | `Assoc (("type", `String "Quantifier") :: ("kind", `String "*") :: ("greedy", `Bool true) :: []) -> Greedy (Star)
+      | `Assoc (("type", `String "Quantifier") :: ("kind", `String "+") :: ("greedy", `Bool true) :: []) -> Greedy (Plus)
+      | `Assoc (("type", `String "Quantifier") :: ("kind", `String "Range") :: ("from", `Int from) :: ("greedy", `Bool true) :: []) -> Greedy (RepPartialRange (from))
+      | `Assoc (("type", `String "Quantifier") :: ("kind", `String "Range") :: ("from", `Int from) :: ("to", `Int until) :: ("greedy", `Bool true) :: []) -> Greedy (RepRange (from, until))
 
-    | `Assoc (("type", `String "Char") :: ("value", `String _) :: ("kind", `String "simple") :: ("symbol", `String _) :: ("codePoint", `Int codepoint) :: ("escaped", `Bool true) :: []) ->
-        AtomEsc (ACharacterEsc (IdentityEsc ((Obj.magic (Warblre.Interop.char_of_int (Obj.magic codepoint))))))
-    | `Assoc (("type", `String "Char") :: ("value", `String _) :: ("kind", `String "simple") :: ("symbol", `String _) :: ("codePoint", `Int codepoint) :: []) -> Char ((Obj.magic (Warblre.Interop.char_of_int (Obj.magic codepoint))))
-    | `Assoc (("type", `String "Char") :: ("value", `String _) :: ("kind", `String "unicode") :: ("symbol", `String _) :: ("codePoint", `Int codepoint) :: []) -> Char ((Obj.magic (Warblre.Interop.char_of_int (Obj.magic codepoint))))
+      | `Assoc (("type", `String "Quantifier") :: ("kind", `String "?") :: ("greedy", `Bool false) :: []) -> Lazy (Question)
+      | `Assoc (("type", `String "Quantifier") :: ("kind", `String "*") :: ("greedy", `Bool false) :: []) -> Lazy (Star)
+      | `Assoc (("type", `String "Quantifier") :: ("kind", `String "+") :: ("greedy", `Bool false) :: []) -> Lazy (Plus)
+      | `Assoc (("type", `String "Quantifier") :: ("kind", `String "Range") :: ("from", `Int from) :: ("greedy", `Bool false) :: []) -> Lazy (RepPartialRange (from))
+      | `Assoc (("type", `String "Quantifier") :: ("kind", `String "Range") :: ("from", `Int from) :: ("to", `Int until) :: ("greedy", `Bool false) :: []) -> Lazy (RepRange (from, until))
 
-    | `Assoc (("type", `String "Char") :: ("value", `String "\\0") :: ("kind", `String "zero") :: []) -> AtomEsc (ACharacterEsc Coq_esc_Zero)
-    | `Assoc (("type", `String "Char") :: ("value", `String ".") :: ("kind", `String "meta") :: ("symbol", `String ".") :: ("codePoint", `Null) :: []) ->
-      Dot
-
-    | `Assoc (("type", `String "Char") :: ("value", `String "\\t") :: ("kind", `String "meta") :: ("symbol", `String _) :: ("codePoint", `Int _) :: []) ->
-      AtomEsc (ACharacterEsc (ControlEsc (Coq_esc_t)))
-    | `Assoc (("type", `String "Char") :: ("value", `String "\\n") :: ("kind", `String "meta") :: ("symbol", `String _) :: ("codePoint", `Int _) :: []) ->
-      AtomEsc (ACharacterEsc (ControlEsc (Coq_esc_n)))
-    | `Assoc (("type", `String "Char") :: ("value", `String "\\f") :: ("kind", `String "meta") :: ("symbol", `String _) :: ("codePoint", `Int _) :: []) ->
-      AtomEsc (ACharacterEsc (ControlEsc (Coq_esc_f)))
-    | `Assoc (("type", `String "Char") :: ("value", `String "\\v") :: ("kind", `String "meta") :: ("symbol", `String _) :: ("codePoint", `Int _) :: []) ->
-      AtomEsc (ACharacterEsc (ControlEsc (Coq_esc_v)))
-    | `Assoc (("type", `String "Char") :: ("value", `String "\\r") :: ("kind", `String "meta") :: ("symbol", `String _) :: ("codePoint", `Int _) :: []) ->
-      AtomEsc (ACharacterEsc (ControlEsc (Coq_esc_r)))
-
-    | `Assoc (("type", `String "Char") :: ("value", `String ctrl) :: ("kind", `String "control") :: []) ->
-      assert(String.length ctrl == 3);
-      AtomEsc (ACharacterEsc (AsciiControlEsc (String.get ctrl 2)))
-    | `Assoc (("type", `String "Char") :: ("value", `String hex) :: ("kind", `String "hex") :: ("symbol", `String _) :: ("codePoint", `Int _) :: []) ->
-      assert(String.length hex == 4);
-      AtomEsc (ACharacterEsc (HexEscape (String.get hex 2, String.get hex 3)))
-
-    | `Assoc (("type", `String "Char") :: ("value", `String "\\s") :: ("kind", `String "meta") :: ("codePoint", `Null) :: []) ->
-      AtomEsc (ACharacterClassEsc (Coq_esc_s))
-    | `Assoc (("type", `String "Char") :: ("value", `String "\\d") :: ("kind", `String "meta") :: ("codePoint", `Null) :: []) ->
-      AtomEsc (ACharacterClassEsc (Coq_esc_d))
-    | `Assoc (("type", `String "Char") :: ("value", `String "\\w") :: ("kind", `String "meta") :: ("codePoint", `Null) :: []) ->
-      AtomEsc (ACharacterClassEsc (Coq_esc_w))
-    | `Assoc (("type", `String "Char") :: ("value", `String "\\S") :: ("kind", `String "meta") :: ("codePoint", `Null) :: []) ->
-      AtomEsc (ACharacterClassEsc (Coq_esc_S))
-    | `Assoc (("type", `String "Char") :: ("value", `String "\\D") :: ("kind", `String "meta") :: ("codePoint", `Null) :: []) ->
-      AtomEsc (ACharacterClassEsc (Coq_esc_D))
-    | `Assoc (("type", `String "Char") :: ("value", `String "\\W") :: ("kind", `String "meta") :: ("codePoint", `Null) :: []) ->
-      AtomEsc (ACharacterClassEsc (Coq_esc_W))
-
-    | `Assoc (("type", `String "CharacterClass") :: ("expressions", `List expressions) :: []) -> CharacterClass (NoninvertedCC (iter_cc expressions))
-    | `Assoc (("type", `String "CharacterClass") :: ("negative", `Bool true) :: ("expressions", `List expressions) :: []) ->
-      CharacterClass (InvertedCC (iter_cc expressions))
-
-    | `Assoc (("type", `String "Disjunction") :: ("left", left) :: ("right", right) :: _) -> Disjunction (iter_r left, iter_r right)
-    | `Assoc (("type", `String "Alternative") :: ("expressions", `List expressions) :: _) -> expressions |> List.map iter_r |> reduce_left (fun l r -> Seq (l, r))
-
-    | `Assoc (("type", `String "Repetition") :: ("expression", expression) :: ("quantifier", quantifier) :: []) -> Quantified (iter_r expression, iter_quantifier quantifier)
-
-    | `Assoc (("type", `String "Group") :: ("capturing", `Bool false) :: ("expression", expression)  :: []) ->
-      iter_r expression
-    | `Assoc (("type", `String "Group") :: ("capturing", `Bool true) :: ("number", `Int _) :: ("expression", expression)  :: []) ->
-      Group (None, iter_r expression)
-    | `Assoc (("type", `String "Group") :: ("capturing", `Bool true) :: ("name", `String name) :: ("nameRaw", `String _) :: ("number", `Int _) :: ("expression", expression)  :: []) ->
-      Group (Some name, iter_r expression)
-
-    | `Assoc (("type", `String "Backreference") :: ("kind", `String "number") :: ("number", `Int i) :: ("reference", `Int _)  :: []) ->
-      AtomEsc (DecimalEsc i)
-    | `Assoc (("type", `String "Backreference") :: ("kind", `String "name") :: ("reference", `String name) :: ("referenceRaw", `String _)  :: []) ->
-      AtomEsc (GroupEsc name)
-
-    | `Assoc (("type", `String "Assertion") :: ("kind", `String "^") :: []) -> InputStart
-    | `Assoc (("type", `String "Assertion") :: ("kind", `String "$") :: []) -> InputEnd
-    | `Assoc (("type", `String "Assertion") :: ("kind", `String "\\b") :: []) -> WordBoundary
-    | `Assoc (("type", `String "Assertion") :: ("kind", `String "\\B") :: []) -> NotWordBoundary
-
-    | `Assoc (("type", `String "Assertion") :: ("kind", `String "Lookahead") :: ("assertion", assertion) :: []) -> Lookahead (iter_r assertion)
-    | `Assoc (("type", `String "Assertion") :: ("kind", `String "Lookahead") :: ("negative", `Bool true) :: ("assertion", assertion) :: []) -> NegativeLookahead (iter_r assertion)
-    | `Assoc (("type", `String "Assertion") :: ("kind", `String "Lookbehind") :: ("assertion", assertion) :: []) -> Lookbehind (iter_r assertion)
-    | `Assoc (("type", `String "Assertion") :: ("kind", `String "Lookbehind") :: ("negative", `Bool true) :: ("assertion", assertion) :: []) -> NegativeLookbehind (iter_r assertion)
-
-    | _ -> failwith (String.cat "Unsupported JSON regex: " (Yojson.Safe.show json)))
-    in
+      | _ -> failwith (String.cat "Unsupported JSON class ranges: " (Yojson.Safe.show json)))
+      in
 
 
-    let string_to_flags str: coq_RegExpFlags =
-        {
-          d = String.contains str 'd';
-          g = String.contains str 'g';
-          i = String.contains str 'i';
-          m = String.contains str 'm';
-          s = String.contains str 's';
-          u = String.contains str 'u';
-          v = String.contains str 'v';
-          y = String.contains str 'y';
-        }
-    in
-    match find_field json "body", find_field json "flags" with
-    | ast, `String flags ->
-        let ast = iter_r ast in
-        let flags = string_to_flags flags in
-        if flags.u then failwith "'u' is not yet supported"
-        else
-          (match (coq_RegExpInitialize ast flags) with
+      let rec iter_r (json: Yojson.Safe.t): coq_Regex = (match json with
+      | `Null -> Empty
+
+      | `Assoc (("type", `String "Char") :: ("value", `String _) :: ("kind", `String "simple") :: ("symbol", `String _) :: ("codePoint", `Int codepoint) :: ("escaped", `Bool true) :: []) ->
+          AtomEsc (ACharacterEsc (IdentityEsc ((Obj.magic (char_of_int codepoint)))))
+      | `Assoc (("type", `String "Char") :: ("value", `String _) :: ("kind", `String "simple") :: ("symbol", `String _) :: ("codePoint", `Int codepoint) :: []) ->
+          Char ((Obj.magic (char_of_int codepoint)))
+      | `Assoc (("type", `String "Char") :: ("value", `String _) :: ("kind", `String "unicode") :: ("symbol", `String _) :: ("codePoint", `Int codepoint) :: []) ->
+          Char ((Obj.magic (char_of_int codepoint)))
+
+      | `Assoc (("type", `String "Char") :: ("value", `String "\\0") :: ("kind", `String "zero") :: []) -> AtomEsc (ACharacterEsc Coq_esc_Zero)
+      | `Assoc (("type", `String "Char") :: ("value", `String ".") :: ("kind", `String "meta") :: ("symbol", `String ".") :: ("codePoint", `Null) :: []) ->
+        Dot
+
+      | `Assoc (("type", `String "Char") :: ("value", `String "\\t") :: ("kind", `String "meta") :: ("symbol", `String _) :: ("codePoint", `Int _) :: []) ->
+        AtomEsc (ACharacterEsc (ControlEsc (Coq_esc_t)))
+      | `Assoc (("type", `String "Char") :: ("value", `String "\\n") :: ("kind", `String "meta") :: ("symbol", `String _) :: ("codePoint", `Int _) :: []) ->
+        AtomEsc (ACharacterEsc (ControlEsc (Coq_esc_n)))
+      | `Assoc (("type", `String "Char") :: ("value", `String "\\f") :: ("kind", `String "meta") :: ("symbol", `String _) :: ("codePoint", `Int _) :: []) ->
+        AtomEsc (ACharacterEsc (ControlEsc (Coq_esc_f)))
+      | `Assoc (("type", `String "Char") :: ("value", `String "\\v") :: ("kind", `String "meta") :: ("symbol", `String _) :: ("codePoint", `Int _) :: []) ->
+        AtomEsc (ACharacterEsc (ControlEsc (Coq_esc_v)))
+      | `Assoc (("type", `String "Char") :: ("value", `String "\\r") :: ("kind", `String "meta") :: ("symbol", `String _) :: ("codePoint", `Int _) :: []) ->
+        AtomEsc (ACharacterEsc (ControlEsc (Coq_esc_r)))
+
+      | `Assoc (("type", `String "Char") :: ("value", `String ctrl) :: ("kind", `String "control") :: []) ->
+        assert(String.length ctrl == 3);
+        AtomEsc (ACharacterEsc (AsciiControlEsc (String.get ctrl 2)))
+      | `Assoc (("type", `String "Char") :: ("value", `String hex) :: ("kind", `String "hex") :: ("symbol", `String _) :: ("codePoint", `Int _) :: []) ->
+        assert(String.length hex == 4);
+        AtomEsc (ACharacterEsc (HexEscape (String.get hex 2, String.get hex 3)))
+
+      | `Assoc (("type", `String "Char") :: ("value", `String "\\s") :: ("kind", `String "meta") :: ("codePoint", `Null) :: []) ->
+        AtomEsc (ACharacterClassEsc (Coq_esc_s))
+      | `Assoc (("type", `String "Char") :: ("value", `String "\\d") :: ("kind", `String "meta") :: ("codePoint", `Null) :: []) ->
+        AtomEsc (ACharacterClassEsc (Coq_esc_d))
+      | `Assoc (("type", `String "Char") :: ("value", `String "\\w") :: ("kind", `String "meta") :: ("codePoint", `Null) :: []) ->
+        AtomEsc (ACharacterClassEsc (Coq_esc_w))
+      | `Assoc (("type", `String "Char") :: ("value", `String "\\S") :: ("kind", `String "meta") :: ("codePoint", `Null) :: []) ->
+        AtomEsc (ACharacterClassEsc (Coq_esc_S))
+      | `Assoc (("type", `String "Char") :: ("value", `String "\\D") :: ("kind", `String "meta") :: ("codePoint", `Null) :: []) ->
+        AtomEsc (ACharacterClassEsc (Coq_esc_D))
+      | `Assoc (("type", `String "Char") :: ("value", `String "\\W") :: ("kind", `String "meta") :: ("codePoint", `Null) :: []) ->
+        AtomEsc (ACharacterClassEsc (Coq_esc_W))
+
+      | `Assoc (("type", `String "CharacterClass") :: ("expressions", `List expressions) :: []) -> CharacterClass (NoninvertedCC (iter_cc expressions))
+      | `Assoc (("type", `String "CharacterClass") :: ("negative", `Bool true) :: ("expressions", `List expressions) :: []) ->
+        CharacterClass (InvertedCC (iter_cc expressions))
+
+      | `Assoc (("type", `String "Disjunction") :: ("left", left) :: ("right", right) :: _) -> Disjunction (iter_r left, iter_r right)
+      | `Assoc (("type", `String "Alternative") :: ("expressions", `List expressions) :: _) -> expressions |> List.map iter_r |> reduce_left (fun l r -> Seq (l, r))
+
+      | `Assoc (("type", `String "Repetition") :: ("expression", expression) :: ("quantifier", quantifier) :: []) -> Quantified (iter_r expression, iter_quantifier quantifier)
+
+      | `Assoc (("type", `String "Group") :: ("capturing", `Bool false) :: ("expression", expression)  :: []) ->
+        iter_r expression
+      | `Assoc (("type", `String "Group") :: ("capturing", `Bool true) :: ("number", `Int _) :: ("expression", expression)  :: []) ->
+        Group (None, iter_r expression)
+      | `Assoc (("type", `String "Group") :: ("capturing", `Bool true) :: ("name", `String name) :: ("nameRaw", `String _) :: ("number", `Int _) :: ("expression", expression)  :: []) ->
+        Group (Some name, iter_r expression)
+
+      | `Assoc (("type", `String "Backreference") :: ("kind", `String "number") :: ("number", `Int i) :: ("reference", `Int _)  :: []) ->
+        AtomEsc (DecimalEsc i)
+      | `Assoc (("type", `String "Backreference") :: ("kind", `String "name") :: ("reference", `String name) :: ("referenceRaw", `String _)  :: []) ->
+        AtomEsc (GroupEsc name)
+
+      | `Assoc (("type", `String "Assertion") :: ("kind", `String "^") :: []) -> InputStart
+      | `Assoc (("type", `String "Assertion") :: ("kind", `String "$") :: []) -> InputEnd
+      | `Assoc (("type", `String "Assertion") :: ("kind", `String "\\b") :: []) -> WordBoundary
+      | `Assoc (("type", `String "Assertion") :: ("kind", `String "\\B") :: []) -> NotWordBoundary
+
+      | `Assoc (("type", `String "Assertion") :: ("kind", `String "Lookahead") :: ("assertion", assertion) :: []) -> Lookahead (iter_r assertion)
+      | `Assoc (("type", `String "Assertion") :: ("kind", `String "Lookahead") :: ("negative", `Bool true) :: ("assertion", assertion) :: []) -> NegativeLookahead (iter_r assertion)
+      | `Assoc (("type", `String "Assertion") :: ("kind", `String "Lookbehind") :: ("assertion", assertion) :: []) -> Lookbehind (iter_r assertion)
+      | `Assoc (("type", `String "Assertion") :: ("kind", `String "Lookbehind") :: ("negative", `Bool true) :: ("assertion", assertion) :: []) -> NegativeLookbehind (iter_r assertion)
+
+      | _ -> failwith (String.cat "Unsupported JSON regex: " (Yojson.Safe.show json)))
+      in
+
+
+      let string_to_flags str: coq_RegExpFlags =
+          {
+            d = String.contains str 'd';
+            g = String.contains str 'g';
+            i = String.contains str 'i';
+            m = String.contains str 'm';
+            s = String.contains str 's';
+            u = String.contains str 'u';
+            v = String.contains str 'v';
+            y = String.contains str 'y';
+          }
+      in
+      match find_field json "body", find_field json "flags" with
+      | ast, `String flags -> (
+          let ast = iter_r ast in
+          let flags = string_to_flags flags in
+          assert (flags.u = false);
+          match (coq_RegExpInitialize ast flags) with
           | Success x -> setLastIndex x index
           | Failure _ -> failwith "Compile error")
-    | _ -> failwith "Invalid JSON regex")
+      | _ -> failwith "Invalid JSON regex")
+end
+
+
+module Unicode = struct
+  open Warblre.Extracted.Patterns
+  open Warblre.Extracted.ECMA_u
+  open Warblre.Interop.Unicode
+
+  let json_to_regex (json: (string * Yojson.Safe.t) list) index: coq_RegExpInstance =
+    Yojson.Safe.(
+      let iter_ca (json: Yojson.Safe.t): coq_ClassAtom = (match json with
+      | `Assoc (("type", `String "Char") :: ("value", `String _) :: ("kind", `String "simple") :: ("symbol", `String _) :: ("codePoint", `Int codepoint) :: ("escaped", `Bool true) :: []) ->
+        ClassEsc (CCharacterEsc (IdentityEsc (Obj.magic (char_of_int codepoint))))
+      | `Assoc (("type", `String "Char") :: ("value", `String _) :: ("kind", `String "simple") :: ("symbol", `String _) :: ("codePoint", `Int codepoint) :: []) ->
+        SourceCharacter ((Obj.magic (char_of_int codepoint)))
+      | `Assoc (("type", `String "Char") :: ("value", `String _) :: ("kind", `String "unicode") :: ("symbol", `String _) :: ("codePoint", `Int codepoint) :: []) ->
+        SourceCharacter ((Obj.magic (char_of_int codepoint)))
+
+      | `Assoc (("type", `String "Char") :: ("value", `String "\\b") :: ("kind", `String "meta") :: ("symbol", `String ".") :: ("codePoint", `Null) :: []) ->
+        ClassEsc(Coq_esc_b)
+      | `Assoc (("type", `String "Char") :: ("value", `String "\\s") :: ("kind", `String "meta") :: ("codePoint", `Null) :: []) ->
+        ClassEsc (CCharacterClassEsc (Coq_esc_s))
+      | `Assoc (("type", `String "Char") :: ("value", `String "\\d") :: ("kind", `String "meta") :: ("codePoint", `Null) :: []) ->
+        ClassEsc (CCharacterClassEsc (Coq_esc_d))
+      | `Assoc (("type", `String "Char") :: ("value", `String "\\w") :: ("kind", `String "meta") :: ("codePoint", `Null) :: []) ->
+        ClassEsc (CCharacterClassEsc (Coq_esc_w))
+      | `Assoc (("type", `String "Char") :: ("value", `String "\\S") :: ("kind", `String "meta") :: ("codePoint", `Null) :: []) ->
+        ClassEsc (CCharacterClassEsc (Coq_esc_S))
+      | `Assoc (("type", `String "Char") :: ("value", `String "\\D") :: ("kind", `String "meta") :: ("codePoint", `Null) :: []) ->
+        ClassEsc (CCharacterClassEsc (Coq_esc_D))
+      | `Assoc (("type", `String "Char") :: ("value", `String "\\W") :: ("kind", `String "meta") :: ("codePoint", `Null) :: []) ->
+        ClassEsc (CCharacterClassEsc (Coq_esc_W))
+
+      | `Assoc (("type", `String "Char") :: ("value", `String "\\t") :: ("kind", `String "meta") :: ("symbol", `String _) :: ("codePoint", `Int _) :: []) ->
+        ClassEsc (CCharacterEsc (ControlEsc (Coq_esc_t)))
+      | `Assoc (("type", `String "Char") :: ("value", `String "\\n") :: ("kind", `String "meta") :: ("symbol", `String _) :: ("codePoint", `Int _) :: []) ->
+        ClassEsc (CCharacterEsc (ControlEsc (Coq_esc_n)))
+      | `Assoc (("type", `String "Char") :: ("value", `String "\\f") :: ("kind", `String "meta") :: ("symbol", `String _) :: ("codePoint", `Int _) :: []) ->
+        ClassEsc (CCharacterEsc (ControlEsc (Coq_esc_f)))
+      | `Assoc (("type", `String "Char") :: ("value", `String "\\v") :: ("kind", `String "meta") :: ("symbol", `String _) :: ("codePoint", `Int _) :: []) ->
+        ClassEsc (CCharacterEsc (ControlEsc (Coq_esc_v)))
+      | `Assoc (("type", `String "Char") :: ("value", `String "\\r") :: ("kind", `String "meta") :: ("symbol", `String _) :: ("codePoint", `Int _) :: []) ->
+        ClassEsc (CCharacterEsc (ControlEsc (Coq_esc_r)))
+
+      | `Assoc (("type", `String "Char") :: ("value", `String ctrl) :: ("kind", `String "control") :: []) ->
+        assert(String.length ctrl == 3);
+        ClassEsc (CCharacterEsc (AsciiControlEsc (String.get ctrl 2)))
+      | `Assoc (("type", `String "Char") :: ("value", `String hex) :: ("kind", `String "hex") :: ("symbol", `String _) :: ("codePoint", `Int _) :: []) ->
+        assert(String.length hex == 4);
+        ClassEsc (CCharacterEsc (HexEscape (String.get hex 2, String.get hex 3)))
+
+      | _  -> failwith (String.cat "Unsupported JSON class atom: " (Yojson.Safe.show json)))
+      in
+
+
+      let rec iter_cc (json: Yojson.Safe.t list): coq_ClassRanges = (match json with
+      | `Assoc (("type", `String "Char") :: r) :: t -> ClassAtomCR (iter_ca (`Assoc (("type", `String "Char") :: r)), iter_cc t)
+
+      | `Assoc (("type", `String "ClassRange") :: ("from", from) :: ("to", until) :: []) :: t->
+        RangeCR (iter_ca from, iter_ca until, iter_cc t)
+
+      | h :: _ -> failwith (String.cat "Unsupported JSON class ranges: " (Yojson.Safe.show h))
+      | [] -> EmptyCR)
+      in
+
+
+      let iter_quantifier (json: Yojson.Safe.t): coq_Quantifier = (match json with
+      | `Assoc (("type", `String "Quantifier") :: ("kind", `String "?") :: ("greedy", `Bool true) :: []) -> Greedy (Question)
+      | `Assoc (("type", `String "Quantifier") :: ("kind", `String "*") :: ("greedy", `Bool true) :: []) -> Greedy (Star)
+      | `Assoc (("type", `String "Quantifier") :: ("kind", `String "+") :: ("greedy", `Bool true) :: []) -> Greedy (Plus)
+      | `Assoc (("type", `String "Quantifier") :: ("kind", `String "Range") :: ("from", `Int from) :: ("greedy", `Bool true) :: []) -> Greedy (RepPartialRange (from))
+      | `Assoc (("type", `String "Quantifier") :: ("kind", `String "Range") :: ("from", `Int from) :: ("to", `Int until) :: ("greedy", `Bool true) :: []) -> Greedy (RepRange (from, until))
+
+      | `Assoc (("type", `String "Quantifier") :: ("kind", `String "?") :: ("greedy", `Bool false) :: []) -> Lazy (Question)
+      | `Assoc (("type", `String "Quantifier") :: ("kind", `String "*") :: ("greedy", `Bool false) :: []) -> Lazy (Star)
+      | `Assoc (("type", `String "Quantifier") :: ("kind", `String "+") :: ("greedy", `Bool false) :: []) -> Lazy (Plus)
+      | `Assoc (("type", `String "Quantifier") :: ("kind", `String "Range") :: ("from", `Int from) :: ("greedy", `Bool false) :: []) -> Lazy (RepPartialRange (from))
+      | `Assoc (("type", `String "Quantifier") :: ("kind", `String "Range") :: ("from", `Int from) :: ("to", `Int until) :: ("greedy", `Bool false) :: []) -> Lazy (RepRange (from, until))
+
+      | _ -> failwith (String.cat "Unsupported JSON class ranges: " (Yojson.Safe.show json)))
+      in
+
+
+      let rec iter_r (json: Yojson.Safe.t): coq_Regex = (match json with
+      | `Null -> Empty
+
+      | `Assoc (("type", `String "Char") :: ("value", `String _) :: ("kind", `String "simple") :: ("symbol", `String _) :: ("codePoint", `Int codepoint) :: ("escaped", `Bool true) :: []) ->
+          AtomEsc (ACharacterEsc (IdentityEsc ((Obj.magic (char_of_int codepoint)))))
+      | `Assoc (("type", `String "Char") :: ("value", `String _) :: ("kind", `String "simple") :: ("symbol", `String _) :: ("codePoint", `Int codepoint) :: []) ->
+          Char ((Obj.magic (char_of_int codepoint)))
+      | `Assoc (("type", `String "Char") :: ("value", `String _) :: ("kind", `String "unicode") :: ("symbol", `String _) :: ("codePoint", `Int codepoint) :: []) ->
+          Char ((Obj.magic (char_of_int codepoint)))
+
+      | `Assoc (("type", `String "Char") :: ("value", `String "\\0") :: ("kind", `String "zero") :: []) -> AtomEsc (ACharacterEsc Coq_esc_Zero)
+      | `Assoc (("type", `String "Char") :: ("value", `String ".") :: ("kind", `String "meta") :: ("symbol", `String ".") :: ("codePoint", `Null) :: []) ->
+        Dot
+
+      | `Assoc (("type", `String "Char") :: ("value", `String "\\t") :: ("kind", `String "meta") :: ("symbol", `String _) :: ("codePoint", `Int _) :: []) ->
+        AtomEsc (ACharacterEsc (ControlEsc (Coq_esc_t)))
+      | `Assoc (("type", `String "Char") :: ("value", `String "\\n") :: ("kind", `String "meta") :: ("symbol", `String _) :: ("codePoint", `Int _) :: []) ->
+        AtomEsc (ACharacterEsc (ControlEsc (Coq_esc_n)))
+      | `Assoc (("type", `String "Char") :: ("value", `String "\\f") :: ("kind", `String "meta") :: ("symbol", `String _) :: ("codePoint", `Int _) :: []) ->
+        AtomEsc (ACharacterEsc (ControlEsc (Coq_esc_f)))
+      | `Assoc (("type", `String "Char") :: ("value", `String "\\v") :: ("kind", `String "meta") :: ("symbol", `String _) :: ("codePoint", `Int _) :: []) ->
+        AtomEsc (ACharacterEsc (ControlEsc (Coq_esc_v)))
+      | `Assoc (("type", `String "Char") :: ("value", `String "\\r") :: ("kind", `String "meta") :: ("symbol", `String _) :: ("codePoint", `Int _) :: []) ->
+        AtomEsc (ACharacterEsc (ControlEsc (Coq_esc_r)))
+
+      | `Assoc (("type", `String "Char") :: ("value", `String ctrl) :: ("kind", `String "control") :: []) ->
+        assert(String.length ctrl == 3);
+        AtomEsc (ACharacterEsc (AsciiControlEsc (String.get ctrl 2)))
+      | `Assoc (("type", `String "Char") :: ("value", `String hex) :: ("kind", `String "hex") :: ("symbol", `String _) :: ("codePoint", `Int _) :: []) ->
+        assert(String.length hex == 4);
+        AtomEsc (ACharacterEsc (HexEscape (String.get hex 2, String.get hex 3)))
+
+      | `Assoc (("type", `String "Char") :: ("value", `String "\\s") :: ("kind", `String "meta") :: ("codePoint", `Null) :: []) ->
+        AtomEsc (ACharacterClassEsc (Coq_esc_s))
+      | `Assoc (("type", `String "Char") :: ("value", `String "\\d") :: ("kind", `String "meta") :: ("codePoint", `Null) :: []) ->
+        AtomEsc (ACharacterClassEsc (Coq_esc_d))
+      | `Assoc (("type", `String "Char") :: ("value", `String "\\w") :: ("kind", `String "meta") :: ("codePoint", `Null) :: []) ->
+        AtomEsc (ACharacterClassEsc (Coq_esc_w))
+      | `Assoc (("type", `String "Char") :: ("value", `String "\\S") :: ("kind", `String "meta") :: ("codePoint", `Null) :: []) ->
+        AtomEsc (ACharacterClassEsc (Coq_esc_S))
+      | `Assoc (("type", `String "Char") :: ("value", `String "\\D") :: ("kind", `String "meta") :: ("codePoint", `Null) :: []) ->
+        AtomEsc (ACharacterClassEsc (Coq_esc_D))
+      | `Assoc (("type", `String "Char") :: ("value", `String "\\W") :: ("kind", `String "meta") :: ("codePoint", `Null) :: []) ->
+        AtomEsc (ACharacterClassEsc (Coq_esc_W))
+
+      | `Assoc (("type", `String "CharacterClass") :: ("expressions", `List expressions) :: []) -> CharacterClass (NoninvertedCC (iter_cc expressions))
+      | `Assoc (("type", `String "CharacterClass") :: ("negative", `Bool true) :: ("expressions", `List expressions) :: []) ->
+        CharacterClass (InvertedCC (iter_cc expressions))
+
+      | `Assoc (("type", `String "Disjunction") :: ("left", left) :: ("right", right) :: _) -> Disjunction (iter_r left, iter_r right)
+      | `Assoc (("type", `String "Alternative") :: ("expressions", `List expressions) :: _) -> expressions |> List.map iter_r |> reduce_left (fun l r -> Seq (l, r))
+
+      | `Assoc (("type", `String "Repetition") :: ("expression", expression) :: ("quantifier", quantifier) :: []) -> Quantified (iter_r expression, iter_quantifier quantifier)
+
+      | `Assoc (("type", `String "Group") :: ("capturing", `Bool false) :: ("expression", expression)  :: []) ->
+        iter_r expression
+      | `Assoc (("type", `String "Group") :: ("capturing", `Bool true) :: ("number", `Int _) :: ("expression", expression)  :: []) ->
+        Group (None, iter_r expression)
+      | `Assoc (("type", `String "Group") :: ("capturing", `Bool true) :: ("name", `String name) :: ("nameRaw", `String _) :: ("number", `Int _) :: ("expression", expression)  :: []) ->
+        Group (Some name, iter_r expression)
+
+      | `Assoc (("type", `String "Backreference") :: ("kind", `String "number") :: ("number", `Int i) :: ("reference", `Int _)  :: []) ->
+        AtomEsc (DecimalEsc i)
+      | `Assoc (("type", `String "Backreference") :: ("kind", `String "name") :: ("reference", `String name) :: ("referenceRaw", `String _)  :: []) ->
+        AtomEsc (GroupEsc name)
+
+      | `Assoc (("type", `String "Assertion") :: ("kind", `String "^") :: []) -> InputStart
+      | `Assoc (("type", `String "Assertion") :: ("kind", `String "$") :: []) -> InputEnd
+      | `Assoc (("type", `String "Assertion") :: ("kind", `String "\\b") :: []) -> WordBoundary
+      | `Assoc (("type", `String "Assertion") :: ("kind", `String "\\B") :: []) -> NotWordBoundary
+
+      | `Assoc (("type", `String "Assertion") :: ("kind", `String "Lookahead") :: ("assertion", assertion) :: []) -> Lookahead (iter_r assertion)
+      | `Assoc (("type", `String "Assertion") :: ("kind", `String "Lookahead") :: ("negative", `Bool true) :: ("assertion", assertion) :: []) -> NegativeLookahead (iter_r assertion)
+      | `Assoc (("type", `String "Assertion") :: ("kind", `String "Lookbehind") :: ("assertion", assertion) :: []) -> Lookbehind (iter_r assertion)
+      | `Assoc (("type", `String "Assertion") :: ("kind", `String "Lookbehind") :: ("negative", `Bool true) :: ("assertion", assertion) :: []) -> NegativeLookbehind (iter_r assertion)
+
+      | _ -> failwith (String.cat "Unsupported JSON regex: " (Yojson.Safe.show json)))
+      in
+
+
+      let string_to_flags str: coq_RegExpFlags =
+          {
+            d = String.contains str 'd';
+            g = String.contains str 'g';
+            i = String.contains str 'i';
+            m = String.contains str 'm';
+            s = String.contains str 's';
+            u = String.contains str 'u';
+            v = String.contains str 'v';
+            y = String.contains str 'y';
+          }
+      in
+      match find_field json "body", find_field json "flags" with
+      | ast, `String flags -> (
+          let ast = iter_r ast in
+          let flags = string_to_flags flags in
+          assert (flags.u = true);
+          match (coq_RegExpInitialize ast flags) with
+          | Success x -> setLastIndex x index
+          | Failure _ -> failwith "Compile error")
+      | _ -> failwith "Invalid JSON regex")
+end
