MECMAR/spec/ECMA.v
@@ -1,4 +1,4 @@
-From Coq Require Import Bool PeanoNat Structures.OrderedType FSets.FSetAVL NArith.
+From Coq Require Import Bool PeanoNat Structures.OrderedType FSets.FSetAVL NArith ZArith.
 From Warblre Require Import Typeclasses Tactics Numeric Characters Patterns RegExp StaticSemantics Semantics List Result Notation Frontend.
 
 Module UInt16.
@@ -7,10 +7,10 @@ Module UInt16.
   Parameter from_numeric_value: non_neg_integer -> type.
   Parameter from_ascii_letter: AsciiLetter -> type.
   Axiom lt : type -> type -> Prop.
-  Parameter compare: type -> type -> nat.
-  Axiom compare_spec_lt: forall l r, Nat.ltb (compare l r) 0 = true -> lt l r.
-  Axiom compare_spec_eq: forall l r, Nat.eqb (compare l r) 0 = true -> eq l r.
-  Axiom compare_spec_gt: forall l r, Nat.ltb 0 (compare l r) = true -> lt r l.
+  Parameter compare: type -> type -> Z.
+  Axiom compare_spec_lt: forall l r, Z.ltb (compare l r) 0 = true -> lt l r.
+  Axiom compare_spec_eq: forall l r, Z.eqb (compare l r) 0 = true -> eq l r.
+  Axiom compare_spec_gt: forall l r, Z.ltb 0 (compare l r) = true -> lt r l.
 
   Axiom numeric_pseudo_bij: forall c, from_numeric_value (numeric_value c) = c.
   Axiom numeric_pseudo_bij2: forall n, n < Pos.to_nat 65536 -> numeric_value (from_numeric_value n) = n.
@@ -30,15 +30,15 @@ Module UInt16.
 
     Definition compare : forall x y : t, Compare lt eq x y.
       intros l r.
-      destruct (Nat.ltb (compare l r) 0) eqn:Lt.
+      destruct (Z.ltb (compare l r) 0) eqn:Lt.
       - apply LT. apply compare_spec_lt. assumption.
-      - destruct (Nat.eqb (compare l r) 0) eqn:Eq.
+      - destruct (Z.eqb (compare l r) 0) eqn:Eq.
         + apply EQ. apply compare_spec_eq. assumption.
-        + assert (forall n m : nat, n <> m -> ~ n < m -> m < n) as H. {
-            intros. apply Lt.nat_total_order_stt in H as [? | ?]; easy.
+        + assert (forall n m : Z, n <> m -> ~ n < m -> m < n)%Z as H. {
+            intros. apply not_Zeq_inf in H as [ ? | ? ]; easy.
           }
-          spec_reflector Nat.ltb_spec0. spec_reflector Nat.eqb_spec.
-          specialize H with (1 := Eq) (2 := Lt). spec_denoter Nat.ltb_spec0.
+          spec_reflector Z.ltb_spec0. spec_reflector Z.eqb_spec.
+          specialize H with (1 := Eq) (2 := Lt). spec_denoter Z.ltb_spec0.
           apply GT. apply compare_spec_gt. assumption.
     Defined.
   End MiniOrdered.
@@ -76,10 +76,72 @@ Module UInt16.
   Parameter digits: list type.
   Parameter white_spaces: list type.
   Parameter ascii_word_characters: list type.
-
 End UInt16.
 
-Module AVLCharSet.
+Module Unicode.
+  Parameter type: Type.
+  Parameter numeric_value: type -> non_neg_integer.
+  Parameter from_numeric_value: non_neg_integer -> type.
+  Parameter from_ascii_letter: AsciiLetter -> type.
+  Axiom lt : type -> type -> Prop.
+  Parameter compare: type -> type -> Z.
+  Axiom compare_spec_lt: forall l r, Z.ltb (compare l r) 0 = true -> lt l r.
+  Axiom compare_spec_eq: forall l r, Z.eqb (compare l r) 0 = true -> eq l r.
+  Axiom compare_spec_gt: forall l r, Z.ltb 0 (compare l r) = true -> lt r l.
+
+  Axiom numeric_pseudo_bij: forall c, from_numeric_value (numeric_value c) = c.
+  Axiom numeric_pseudo_bij2: forall n, n < Pos.to_nat 65536 -> numeric_value (from_numeric_value n) = n.
+
+  Module MiniOrdered <: MiniOrderedType.
+    Definition t := type.
+
+    Definition eq : t -> t -> Prop := Logic.eq.
+    Definition lt : t -> t -> Prop := Unicode.lt.
+
+    Axiom eq_refl : forall x : t, eq x x.
+    Axiom eq_sym : forall x y : t, eq x y -> eq y x.
+    Axiom eq_trans : forall x y z : t, eq x y -> eq y z -> eq x z.
+
+    Axiom lt_trans : forall x y z : t, lt x y -> lt y z -> lt x z.
+    Axiom lt_not_eq : forall x y : t, lt x y -> ~ eq x y.
+
+    Definition compare : forall x y : t, Compare lt eq x y.
+      intros l r.
+      destruct (Z.ltb (compare l r) 0) eqn:Lt.
+      - apply LT. apply compare_spec_lt. assumption.
+      - destruct (Z.eqb (compare l r) 0) eqn:Eq.
+        + apply EQ. apply compare_spec_eq. assumption.
+        + assert (forall n m : Z, n <> m -> ~ n < m -> m < n)%Z as H. {
+            intros. apply not_Zeq_inf in H as [ ? | ? ]; easy.
+          }
+          spec_reflector Z.ltb_spec0. spec_reflector Z.eqb_spec.
+          specialize H with (1 := Eq) (2 := Lt). spec_denoter Z.ltb_spec0.
+          apply GT. apply compare_spec_gt. assumption.
+    Defined.
+  End MiniOrdered.
+  Module Ordered := MOT_to_OT (MiniOrdered).
+  #[export] Instance eqdec_uint16: EqDec type := { eq_dec := Ordered.eq_dec; }.
+
+  Parameter CodePoint: Type.
+  Parameter case_fold: type -> type.
+
+  Definition canonicalize (rer: RegExp) (ch: type): type :=
+    (* 1. If rer.[[Unicode]] is true and rer.[[IgnoreCase]] is true, then *)
+    if (RegExp.ignoreCase rer == true) then
+      (* a. a. If the file CaseFolding.txt of the Unicode Character Database provides a simple or common case folding mapping for ch, return the result of applying that mapping to ch. *)
+      (* b. Return ch. *)
+      case_fold ch
+    (* 2. If rer.[[IgnoreCase]] is false, return ch. *)
+    else ch.
+
+  Parameter all: list type.
+  Parameter line_terminators: list type.
+  Parameter digits: list type.
+  Parameter white_spaces: list type.
+  Parameter ascii_word_characters: list type.
+End Unicode.
+
+Module AVL_UInt16_CharSet.
   Module M := Make (UInt16.Ordered).
 
   Local Definition from_list := fun ls => List.fold_left (fun s c => M.add c s) ls M.empty.
@@ -107,7 +169,37 @@ Module AVLCharSet.
     exist := fun s (m: UInt16.type -> bool) => M.exists_ m s;
   }.
   Proof. - reflexivity. - reflexivity. Defined.
-End AVLCharSet.
+End AVL_UInt16_CharSet.
+
+Module AVL_Unicode_CharSet.
+  Module M := Make (Unicode.Ordered).
+
+  Local Definition from_list := fun ls => List.fold_left (fun s c => M.add c s) ls M.empty.
+
+  #[refine]
+  Instance instance: @CharSet.class Unicode.type := {
+    set_type := M.t;
+
+    empty := M.empty;
+    from_list := from_list;
+    union := fun l r => M.union l r;
+    singleton := fun c => M.singleton c;
+    size := fun s => M.cardinal s;
+    remove_all := fun l r => M.diff l r;
+
+    is_empty := fun s => M.is_empty s;
+
+    contains := fun s c => M.mem c s;
+
+    range := fun l h => from_list (List.map Unicode.from_numeric_value (List.Range.Nat.Bounds.range (Unicode.numeric_value l) (S (Unicode.numeric_value h))));
+
+    unique := fun {F: Type} {_: Result.AssertionError F} s =>
+      if (Nat.eqb (M.cardinal s) 1) then Result.Conversions.from_option (M.choose s) else Result.assertion_failed;
+    filter := fun s (f: Unicode.type -> bool) => M.filter f s;
+    exist := fun s (m: Unicode.type -> bool) => M.exists_ m s;
+  }.
+  Proof. - reflexivity. - reflexivity. Defined.
+End AVL_Unicode_CharSet.
 
 Module Utf16CharCode.
   #[refine]
@@ -119,7 +211,7 @@ Module Utf16CharCode.
     numeric_value := UInt16.numeric_value;
     canonicalize := UInt16.canonicalize;
 
-    set_type := AVLCharSet.instance;
+    set_type := AVL_UInt16_CharSet.instance;
 
     (* Some important (sets of) characters *)
     all := UInt16.all;
@@ -130,6 +222,28 @@ Module Utf16CharCode.
   }.
   Proof. - apply UInt16.numeric_pseudo_bij. - apply UInt16.numeric_pseudo_bij2. Defined.
 End Utf16CharCode.
+
+Module UnicodeCharCode.
+  #[refine]
+  Instance instance: Character.class := {
+    (* The character type and its operations *)
+    type := Unicode.type;
+    eq_dec := Unicode.eqdec_uint16;
+    from_numeric_value := Unicode.from_numeric_value;
+    numeric_value := Unicode.numeric_value;
+    canonicalize := Unicode.canonicalize;
+
+    set_type := AVL_Unicode_CharSet.instance;
+
+    (* Some important (sets of) characters *)
+    all := Unicode.all;
+    line_terminators := Unicode.line_terminators;
+    digits := Unicode.digits;
+    white_spaces := Unicode.white_spaces;
+    ascii_word_characters := Unicode.ascii_word_characters;
+  }.
+  Proof. - apply Unicode.numeric_pseudo_bij. - apply Unicode.numeric_pseudo_bij2. Defined.
+End UnicodeCharCode.
 
 Module Type Parameters.
   Parameter char_instance: @Character.class.
@@ -181,3 +295,11 @@ End ECMASig.
 Module ECMA.
   Include Instance ECMASig.
 End ECMA.
+
+Module ECMASig_u <: Parameters.
+  Definition char_instance: @Character.class := UnicodeCharCode.instance.
+  Definition Character: Type := Unicode.type.
+End ECMASig_u.
+Module ECMA_u.
+  Include Instance ECMASig_u.
+End ECMA_u.
