extraction/Extraction.v
@@ -14,23 +14,36 @@ Extract Constant HexDigit.to_integer => "Interop.parse_hex".
 Extract Constant AsciiLetter.type => "char".
 Extract Constant AsciiLetter.numeric_value => "Char.code".
 
-Extract Constant UInt16.all => "Interop.all_chars".
-Extract Constant UInt16.line_terminators => "Interop.line_terminators".
-Extract Constant UInt16.white_spaces => "Interop.white_spaces".
-Extract Constant UInt16.digits => "Interop.digits".
-Extract Constant UInt16.ascii_word_characters => "Interop.ascii_word_characters".
-
 Extract Constant Patterns.GroupName => "string".
 Extract Constant Patterns.GroupName_eq_dec => "String.equal".
 
-Extract Constant UInt16.code_points_to_string => "Interop.code_points_to_string".
-Extract Constant UInt16.to_upper_case => "Interop.to_upper_case".
-Extract Constant UInt16.type => "Interop.character".
-Extract Constant UInt16.to_code_point => "Interop.code_point".
-Extract Constant UInt16.CodePoint => "Interop.codepoint".
-Extract Constant UInt16.numeric_value => "Interop.char_to_int".
-Extract Constant UInt16.from_numeric_value => "Interop.char_of_int".
-Extract Constant UInt16.compare => "Interop.cmp".
+Extract Constant UInt16.code_points_to_string => "Interop.Utf16.code_points_to_string".
+Extract Constant UInt16.to_upper_case => "Interop.Utf16.to_upper_case".
+Extract Constant UInt16.type => "Interop.Utf16.character".
+Extract Constant UInt16.to_code_point => "Interop.Utf16.code_point".
+Extract Constant UInt16.CodePoint => "Interop.Utf16.codepoint".
+Extract Constant UInt16.numeric_value => "Interop.Utf16.char_to_int".
+Extract Constant UInt16.from_numeric_value => "Interop.Utf16.char_of_int".
+Extract Constant UInt16.compare => "Interop.Utf16.cmp".
 
-Extraction "Extracted.ml" RegExp.RegExp  ECMA.ECMA.
+Extract Constant UInt16.all => "Interop.Utf16.all_chars".
+Extract Constant UInt16.line_terminators => "Interop.Utf16.line_terminators".
+Extract Constant UInt16.white_spaces => "Interop.Utf16.white_spaces".
+Extract Constant UInt16.digits => "Interop.Utf16.digits".
+Extract Constant UInt16.ascii_word_characters => "Interop.Utf16.ascii_word_characters".
+
+
+Extract Constant Unicode.type => "Interop.Unicode.character".
+Extract Constant Unicode.numeric_value => "Interop.Unicode.char_to_int".
+Extract Constant Unicode.from_numeric_value => "Interop.Unicode.char_of_int".
+Extract Constant Unicode.compare => "Interop.Unicode.cmp".
+Extract Constant Unicode.case_fold => "Interop.Unicode.case_fold".
+
+Extract Constant Unicode.all => "Interop.Unicode.all_chars".
+Extract Constant Unicode.line_terminators => "Interop.Unicode.line_terminators".
+Extract Constant Unicode.white_spaces => "Interop.Unicode.white_spaces".
+Extract Constant Unicode.digits => "Interop.Unicode.digits".
+Extract Constant Unicode.ascii_word_characters => "Interop.Unicode.ascii_word_characters".
+
+Extraction "Extracted.ml" RegExp.RegExp  ECMA.ECMA ECMA.ECMA_u.
 
